Refactor several things

src/Schema.v
@@ -8,6 +8,8 @@ From extructures Require Import ord.
 Require Import treeordtype.
 
 
+Delimit Scope schema_scope with SCHEMA.
+Open Scope schema_scope.
 
 Section Schema.
 
@@ -16,130 +18,51 @@ Section Schema.
       https://facebook.github.io/graphql/June2018/#sec-Names **)
   Variable Name : ordType.
 
-
+  
   (** Same as names, except that it can't be true, false or null. 
       Right now it is just the same as Name.
 
       https://facebook.github.io/graphql/June2018/#EnumValue **)
   Definition EnumValue := Name.
 
-  Definition NamedType := Name.
 
-  (** Types of data expected by query variables.
+  
+  Section Types.
+    Definition NamedType := Name.
 
-      https://facebook.github.io/graphql/June2018/#sec-Type-References **)
-  Inductive type : Type :=
-  | NT : NamedType -> type
-  | ListType : type -> type.
+    (** Types of data expected by query variables.
+
+        https://facebook.github.io/graphql/June2018/#sec-Type-References
+     **)
+    Inductive type : Type :=
+    | NT : NamedType -> type
+    | ListType : type -> type.
+
 
 
   
-  (** Get a type's wrapped name.
-      Corresponds to a named type's actual name or the name used in a list type
+    (** Get a type's wrapped name.
+        Corresponds to a named type's actual name or the name used in a list type
 
-      https://facebook.github.io/graphql/June2018/#sec-Type-References
-      https://facebook.github.io/graphql/June2018/#sec-Wrapping-Types
-   **)
-  Fixpoint name_of_type (ty : type) : Name :=
-    match ty with
-    | NT name => name
-    | ListType ty' => name_of_type ty'
-    end.
+        https://facebook.github.io/graphql/June2018/#sec-Type-References
+        https://facebook.github.io/graphql/June2018/#sec-Wrapping-Types
+     **)
+    Fixpoint name_of_type (ty : type) : Name :=
+      match ty with
+      | NT name => name
+      | ListType ty' => name_of_type ty'
+      end.
 
-  Coercion name_of_type : type >-> Ord.sort.
-
-  
-  (** Argument for a field.
-
-      In the specification it is named "InputValue" (InputValueDefinition) but 
-      it is not very descriptive of what it is. Besides, it is constantly refered 
-      as "argument", therefore it is named as FieldArgument (only fields can have
-      arguments so it may sound redundant to name it like this but I feel it is
-      more descriptive and reinforces this notion). 
-
-      https://facebook.github.io/graphql/June2018/#sec-Field-Arguments **)
-  Inductive FieldArgumentDefinition : Type :=
-  | FieldArgument : Name -> type -> FieldArgumentDefinition.
+    Coercion name_of_type : type >-> Ord.sort.
 
 
-  Definition name_of_argument (arg : FieldArgumentDefinition) := let: FieldArgument n _ := arg in n.
-  Definition type_of_argument (arg : FieldArgumentDefinition) := let: FieldArgument _ ty := arg in ty.
- 
-  
-  (** https://facebook.github.io/graphql/June2018/#FieldDefinition **)
-  Inductive FieldDefinition : Type :=
-  | Field : Name -> seq FieldArgumentDefinition -> type -> FieldDefinition.
-
-
-  Definition name_of_field (fld : FieldDefinition) : Name :=
-    let: Field n _ _ := fld in n.
-  Definition type_of_field (fld : FieldDefinition) : type :=
-    let: Field _ _ ty := fld in ty.
-
-  Coercion type_of_field : FieldDefinition >-> type.
-
-  (** Possible type definitions one can make in a GraphQL service. Some observations:
-
-    1. Objects' interfaces: Objects *may* declare one or more implemented interfaces. This is 
-    is implemented as a list of <type>, which can be empty or not. As it is, an
-    object may declare an interface as a list type (eg. "type A implements [B]"), therefore
-    in the wf property there is a check that restricts this declaration to a 
-    named type.
-
-    2. Fields: Objects and interfaces must declare at least one field but the current
-    definition allows an empty list of fields. In the wf property it is checked that
-    this list is not empty.
-
-    3. InputObjects: Currently not included to simplify the formalization.
-
-
-    https://facebook.github.io/graphql/June2018/#TypeDefinition
-   **)
-
-  Inductive TypeDefinition : Type :=
-  | ScalarTypeDefinition : Name -> TypeDefinition
-  | ObjectTypeDefinition : Name -> seq NamedType -> seq FieldDefinition -> TypeDefinition
-  | InterfaceTypeDefinition : Name -> seq FieldDefinition -> TypeDefinition
-  | UnionTypeDefinition : Name -> seq NamedType -> TypeDefinition
-  | EnumTypeDefinition : Name -> seq EnumValue -> TypeDefinition.
-  
-
-  (** 
-      The Schema corresponds to the type system - the collective types defined and a
-      reference to the Query type (the entry point for queries).
-
-      This differs from the Schema mentioned in the specification. I believe there is
-      some naming clashes when they refer to a Schema:
- 
-          A GraphQL service’s collective type system capabilities are referred to as
-          that service’s “schema”. A schema is defined in terms of the types and 
-          directives it supports as well as the root operation types for each kind of
-          operation: query, mutation, and subscription [...]
-
-    This description matches the definition given in this file, but one can also define 
-    a "schema", which only describes the types for the operations: query, mutation and suscription.
-
-
-
-   **)
-  Structure schema := Schema {
-                      query_type : NamedType;
-                      typeDefinitions : seq TypeDefinition
-                    }.
-
-
-  
- 
-    (** Establishing eqType for different structures: type, arguments, fields **)
-
-    
     (** Get a tree out of a type **)
     Fixpoint tree_of_type (ty : type) : GenTree.tree Name :=
       match ty with
       | NT n => GenTree.Node 0 [:: GenTree.Leaf n]
       | ListType ty' => GenTree.Node 1 [:: tree_of_type ty']
       end.
-
+      
     (** Get a type out of a tree or none **)
     Fixpoint type_of_tree (t : GenTree.tree Name) : option type :=
       match t with
@@ -150,71 +73,233 @@ Section Schema.
                                    None
       | _ => None
       end.
-
+      
     Lemma pcan_tree_of_type : pcancel tree_of_type type_of_tree.
-    Proof. 
-        by elim=> [| t /= ->].
-    Qed.
-
+    Proof. by elim=> [| t /= ->]. Qed.
+    
     Definition type_eqMixin := PcanEqMixin pcan_tree_of_type.
     Canonical type_eqType := EqType type type_eqMixin.
     Definition type_choiceMixin := PcanChoiceMixin pcan_tree_of_type.
     Canonical type_choiceType := ChoiceType type type_choiceMixin.
-
+    
     Definition type_ordMixin := PcanOrdMixin pcan_tree_of_type.
     Canonical type_ordType := OrdType type type_ordMixin.
+      
+  End Types.
+
+
+
+  Section TypeSystem.
+
+    
+    (** Argument for a field.
+
+        In the specification it is named "InputValue" (InputValueDefinition) but 
+        it is not very descriptive of what it is. Besides, it is constantly refered 
+        as "argument", therefore it is named as FieldArgument (only fields can have
+        arguments so it may sound redundant to name it like this but I feel it is
+        more descriptive and reinforces this notion). 
+
+        https://facebook.github.io/graphql/June2018/#sec-Field-Arguments **)
+    Record FieldArgumentDefinition := FieldArgument {
+                                         argname : Name;
+                                         argtype : type
+                                       }.
+  
+    (** https://facebook.github.io/graphql/June2018/#FieldDefinition **)
+    Record FieldDefinition := Field {
+                                 field_name : Name;
+                                 args : seq FieldArgumentDefinition;
+                                 return_type : type
+                               }.
+
+
+    (** Possible type definitions one can make in a GraphQL service. Some observations:
+
+        1. Objects' interfaces: Objects *may* declare one or more implemented interfaces. This is 
+        is implemented as a list of <type>, which can be empty or not. As it is, an
+        object may declare an interface as a list type (eg. "type A implements [B]"), therefore
+        in the wf property there is a check that restricts this declaration to a 
+        named type.
+
+        2. Fields: Objects and interfaces must declare at least one field but the current
+        definition allows an empty list of fields. In the wf property it is checked that
+        this list is not empty.
+
+        3. InputObjects: Currently not included to simplify the formalization.
+
+
+        https://facebook.github.io/graphql/June2018/#TypeDefinition
+     **)
+
+    Inductive TypeDefinition : Type :=
+    | ScalarTypeDefinition : Name -> TypeDefinition
+    | ObjectTypeDefinition : Name -> seq NamedType -> seq FieldDefinition -> TypeDefinition
+    | InterfaceTypeDefinition : Name -> seq FieldDefinition -> TypeDefinition
+    | UnionTypeDefinition : Name -> seq NamedType -> TypeDefinition
+    | EnumTypeDefinition : Name -> seq EnumValue -> TypeDefinition.
     
 
+    (** 
+        The Schema corresponds to the type system - the collective types defined and a
+        reference to the Query type (the entry point for queries).
 
-    Definition prod_of_arg (arg : FieldArgumentDefinition) := let: FieldArgument n t := arg in (n, t).
-    Definition arg_of_prod (p : prod Name type) := let: (n, t) := p in FieldArgument n t.
+        This differs from the Schema mentioned in the specification. I believe there is
+        some naming clashes when they refer to a Schema:
+ 
+        A GraphQL service’s collective type system capabilities are referred to as
+        that service’s “schema”. A schema is defined in terms of the types and 
+        directives it supports as well as the root operation types for each kind of
+        operation: query, mutation, and subscription [...]
 
-    Lemma prod_of_argK : cancel prod_of_arg arg_of_prod.
-    Proof. by case. Qed.
-
-    Definition arg_eqMixin := CanEqMixin prod_of_argK.
-    Canonical arg_eqType := EqType FieldArgumentDefinition arg_eqMixin.
-
-
-
-    Definition prod_of_field (f : FieldDefinition) := let: Field n args t := f in (n, args, t).
-    Definition field_of_prod (p : Name * (seq.seq FieldArgumentDefinition) * type)  := let: (n, args, t) := p in Field n args t.
-
-    Lemma prod_of_fieldK : cancel prod_of_field field_of_prod.
-    Proof. by case. Qed.
-
-    Definition field_eqMixin := CanEqMixin prod_of_fieldK.
-    Canonical field_eqType := EqType FieldDefinition field_eqMixin.
+        This description matches the definition given in this file, but one can also define 
+        a "schema", which only describes the types for the operations: query, mutation and suscription.
+   **)
+    Record schema := Schema {
+                        query_type : NamedType;
+                        typeDefinitions : seq TypeDefinition
+                      }.
 
 
-    Definition type_definition_eq tdef1 tdef2 :=
-      match tdef1, tdef2 with
-      | ScalarTypeDefinition n, ScalarTypeDefinition n' => n == n'
-      | ObjectTypeDefinition n tys flds, ObjectTypeDefinition n' tys' flds' => [&& (n == n'), (tys == tys') & (flds == flds')]
-      | InterfaceTypeDefinition n flds, InterfaceTypeDefinition n' flds' => (n == n') && (flds == flds')
-      | UnionTypeDefinition n mbs, UnionTypeDefinition n' mbs' => (n == n') && (mbs == mbs')
-      | EnumTypeDefinition n es, EnumTypeDefinition n' es' => (n == n') && (es == es')
-      | _, _ => false
-      end.
+  End TypeSystem.
+
+ 
+      
+  Definition prod_of_arg (arg : FieldArgumentDefinition) := let: FieldArgument n t := arg in (n, t).
+  Definition arg_of_prod (p : prod Name type) := let: (n, t) := p in FieldArgument n t.
+
+  Lemma prod_of_argK : cancel prod_of_arg arg_of_prod.  Proof. by case. Qed.
+  
+  Definition arg_eqMixin := CanEqMixin prod_of_argK.
+  Canonical arg_eqType := EqType FieldArgumentDefinition arg_eqMixin.
   
 
+  
+  Coercion return_type : FieldDefinition >-> type.
+  
+  Definition prod_of_field (f : FieldDefinition) := let: Field n args t := f in (n, args, t).
+  Definition field_of_prod (p : Name * (seq.seq FieldArgumentDefinition) * type)  := let: (n, args, t) := p in Field n args t.
+  
+  Lemma prod_of_fieldK : cancel prod_of_field field_of_prod. Proof. by case. Qed.
+  
+  Definition field_eqMixin := CanEqMixin prod_of_fieldK.
+  Canonical field_eqType := EqType FieldDefinition field_eqMixin.
 
-    Lemma type_definition_eqP : Equality.axiom type_definition_eq.
-    Proof.
-      move=> t1 t2; apply: (iffP idP) => [|<-].
-      elim: t1; elim: t2 => //.
-        by move=> n n' /= /eqP => ->.
-        by move=> n tyzs flds n' tys' flds' /=; case/and3P=> /eqP -> /eqP -> /eqP ->.
-        by move=> n flds n' flds' /=; move/andP=> [/eqP -> /eqP ->].  
-        by move=> n mbs n' mbs'; move/andP=> [/eqP -> /eqP ->].
-        by move=> n es n' es'; move/andP=> [/eqP -> /eqP ->].
-      by elim: t1; move=> * /=; rewrite !eqxx.
-    Qed.
 
-    Definition type_definition_eqMixin := EqMixin type_definition_eqP.
-    Canonical type_definition_eqType := EqType TypeDefinition type_definition_eqMixin.
+
+   
+  Fixpoint name_of_type_definition tdef : Name :=
+    match tdef with 
+    | ScalarTypeDefinition name => name
+    | ObjectTypeDefinition name _ _ => name
+    | InterfaceTypeDefinition name _ => name
+    | UnionTypeDefinition name _ => name
+    | EnumTypeDefinition name _ => name
+    end.
+  
+  Coercion name_of_type_definition : TypeDefinition >-> Ord.sort.
+
+  
+  Definition type_definition_eq tdef1 tdef2 :=
+    match tdef1, tdef2 with
+    | ScalarTypeDefinition n, ScalarTypeDefinition n' => n == n'
+    | ObjectTypeDefinition n tys flds, ObjectTypeDefinition n' tys' flds' => [&& (n == n'), (tys == tys') & (flds == flds')]
+    | InterfaceTypeDefinition n flds, InterfaceTypeDefinition n' flds' => (n == n') && (flds == flds')
+    | UnionTypeDefinition n mbs, UnionTypeDefinition n' mbs' => (n == n') && (mbs == mbs')
+    | EnumTypeDefinition n es, EnumTypeDefinition n' es' => (n == n') && (es == es')
+    | _, _ => false
+    end.
+  
+
+  Lemma type_definition_eqP : Equality.axiom type_definition_eq.
+  Proof.
+    move=> t1 t2; apply: (iffP idP) => [|<-].
+    elim: t1; elim: t2 => //.
+      by move=> n n' /= /eqP => ->.
+      by move=> n tyzs flds n' tys' flds' /=; case/and3P=> /eqP -> /eqP -> /eqP ->.
+      by move=> n flds n' flds' /= /andP [/eqP -> /eqP ->].  
+      by move=> n mbs n' mbs' /andP [/eqP -> /eqP ->].
+      by move=> n es n' es' /andP [/eqP -> /eqP ->].
+    by elim: t1; move=> * /=; rewrite !eqxx.
+  Qed.
+
+    
+  Definition type_definition_eqMixin := EqMixin type_definition_eqP.
+  Canonical type_definition_eqType := EqType TypeDefinition type_definition_eqMixin.
+
+
+  
+
+  Definition prod_of_schema (s : schema) := let: Schema q tdefs := s in (q, tdefs).
+  Definition schema_of_prod p := let: (q, tdefs) := p in Schema q tdefs.
+
+  Lemma prod_of_schemaK : cancel prod_of_schema schema_of_prod.  Proof. by case. Qed.
+  
+  Definition schema_eqMixin := CanEqMixin prod_of_schemaK.
+  Canonical schema_eqType := EqType schema schema_eqMixin.
+  
       
+  Definition fun_of_schema (s : schema) : TypeDefinition -> bool := fun tdef => tdef \in s.(typeDefinitions).
+  Coercion fun_of_schema : schema >-> Funclass.
+  Coercion typeDefinitions : schema >-> seq.
+
+
+  Lemma in_schemaE (s : schema) tdef : s tdef = (tdef \in s.(typeDefinitions)).
+  Proof. done. Qed.
+    
+  Definition is_named tdef name : bool :=
+    match tdef with
+    | ScalarTypeDefinition n => n == name
+    | ObjectTypeDefinition n _ _ => n == name
+    | InterfaceTypeDefinition n _ => n == name
+    | UnionTypeDefinition n _ => n == name
+    | EnumTypeDefinition n _ => n == name
+    end.
+  
+  Definition pred_of_schema (s : schema) : collective_pred Name :=
+    [pred ty : Name | has (fun tdef => is_named tdef ty) s.(typeDefinitions)].
+  
+  Canonical schema_predType := mkPredType pred_of_schema.
+  
+  Definition tdef_pred_of_schema (s : schema) :=
+    [pred tdef : TypeDefinition | tdef \in s.(typeDefinitions)].
+    
+    
+  Lemma name_in_schemaE (s : schema) (n : Name) : n \in s = has (fun tdef => is_named tdef n) s.
+  Proof. done. Qed.
+    
+     
+  Definition contains_field_name tdef (name : Name) : bool :=
+    match tdef with
+    | ScalarTypeDefinition _ => false
+    | ObjectTypeDefinition n _ flds => has (fun fld => fld.(field_name) == name) flds
+    | InterfaceTypeDefinition n flds => has (fun fld => fld.(field_name) == name) flds
+    | UnionTypeDefinition n mbs => name \in mbs
+    | EnumTypeDefinition n evs => name \in evs
+    end.
+    
+    Definition pred_of_type_definition (tdef : TypeDefinition) : collective_pred Name :=
+      [pred ty : Name | contains_field_name tdef ty].
+  
+    Canonical type_definition_predType := mkPredType pred_of_type_definition.
+    
+    Lemma in_typeDefinitionE (tdef : TypeDefinition) (n : Name) : n \in tdef = contains_field_name tdef n.
+    Proof. done. Qed.
+    
+    
 End Schema.
+
+
+
+Notation "[ name ]" := (ListType name).
+Notation "argname : ty" := (FieldArgument argname ty) : schema_scope.
+Notation "fname '(' args ')' ':' ty" := (Field fname args ty) (at level 50) : schema_scope.
+Notation "'scalar' S" := (ScalarTypeDefinition S) (at level 0) : schema_scope.
+Notation "'object' O '{' flds '}'" := (ObjectTypeDefinition O [::] flds) : schema_scope.
+Notation "'object' O 'implements' I '{' flds '}'" := (ObjectTypeDefinition O I flds) : schema_scope.
+Notation "'interface' I '{' flds '}'" := (InterfaceTypeDefinition I flds) : schema_scope.
+Notation "'union' U '{' mbs '}'" := (UnionTypeDefinition U mbs) : schema_scope.
+Notation "'enum' E '{' evs '}'" := (EnumTypeDefinition E evs) : schema_scope.
 
 Arguments NamedType [Name].
 Arguments type [Name].
@@ -224,9 +309,3 @@ Arguments TypeDefinition [Name].
 Arguments Schema [Name].
 
 Arguments name_of_type [Name].
-
-Arguments name_of_argument [Name].
-Arguments type_of_argument [Name].
-
-Arguments name_of_field [Name].
-Arguments type_of_field [Name].
